fstar/test/MLS.Test.FromExt.MessageProtection.fst
@@ -1,0 +1,144 @@
+module MLS.Test.FromExt.MessageProtection
+
+open FStar.IO
+open FStar.All
+open Comparse
+open MLS.Test.Types
+open MLS.Test.Utils
+open MLS.StringUtils
+
+open Comparse
+open MLS.Result
+open MLS.NetworkTypes
+open MLS.Crypto
+open MLS.TreeDEM.NetworkTypes
+open MLS.TreeDEM.Message.Framing
+
+val gen_group_context: {|bytes_like bytes|} -> message_protection_test -> ML bytes
+let gen_group_context t =
+  let cipher_suite = available_ciphersuite_to_network (extract_result (uint16_to_ciphersuite t.cipher_suite)) in
+  let group_id = hex_string_to_bytes t.group_id in
+  let epoch = FStar.UInt64.v t.epoch in
+  let tree_hash = hex_string_to_bytes t.tree_hash in
+  let confirmed_transcript_hash = hex_string_to_bytes t.confirmed_transcript_hash in
+  if length group_id < pow2 30 && epoch < (pow2 64) && length tree_hash < pow2 30 && length confirmed_transcript_hash < pow2 30 then (
+    (ps_prefix_to_ps_whole ps_group_context_nt).serialize ({
+      version = PV_mls10;
+      cipher_suite;
+      group_id;
+      epoch;
+      tree_hash;
+      confirmed_transcript_hash;
+      extensions = [];
+    })
+  ) else (
+    failwith "gen_group_context: bad data"
+  )
+
+val extract_public_message: {|bytes_like bytes|} -> string -> ML (public_message_nt bytes)
+let extract_public_message #bl s =
+  match parse (mls_message_nt bytes) (hex_string_to_bytes s) with
+  | None -> failwith "extract_public_message: not a parseable mls_message"
+  | Some (M_mls10 (M_public_message res)) -> res
+  | Some _ -> failwith "extract_public_message: not a public message"
+
+val extract_private_message: {|bytes_like bytes|} -> string -> ML (private_message_nt bytes)
+let extract_private_message #bl s =
+  match parse (mls_message_nt bytes) (hex_string_to_bytes s) with
+  | None -> failwith "extract_private_message: not a parseable mls_message"
+  | Some (M_mls10 (M_private_message res)) -> res
+  | Some _ -> failwith "extract_private_message: not a private message"
+
+val extract_proposal: {|bytes_like bytes|} -> authenticated_content_nt bytes -> ML (proposal_nt bytes)
+let extract_proposal #bl content =
+  match content.content.content.content_type with
+  | CT_proposal -> content.content.content.content
+  | _ -> failwith "extract_proposal: not a proposal"
+
+val test_proposal_protection: {|crypto_bytes bytes|} -> message_protection_test -> ML bool
+let test_proposal_protection #cb t =
+  let encryption_secret = hex_string_to_bytes t.encryption_secret in
+  let sender_data_secret = hex_string_to_bytes t.sender_data_secret in
+  let proposal = hex_string_to_bytes t.proposal in
+  let proposal_pub = extract_public_message t.proposal_pub in
+  let proposal_priv = extract_private_message t.proposal_priv in
+
+  let the_proposal_pub = extract_proposal (message_plaintext_to_message proposal_pub) in
+  let the_proposal_priv = extract_proposal (extract_result (message_ciphertext_to_message 1 encryption_secret sender_data_secret proposal_priv)) in
+
+  let the_proposal_pub_ok = check_equal "proposal_pub" (bytes_to_hex_string) (proposal) ((ps_prefix_to_ps_whole ps_proposal_nt).serialize the_proposal_pub) in
+  let the_proposal_priv_ok = check_equal "proposal_priv" (bytes_to_hex_string) (proposal) ((ps_prefix_to_ps_whole ps_proposal_nt).serialize the_proposal_priv) in
+
+  the_proposal_pub_ok && the_proposal_priv_ok
+
+val extract_commit: {|bytes_like bytes|} -> authenticated_content_nt bytes -> ML (commit_nt bytes)
+let extract_commit #bl content =
+  match content.content.content.content_type with
+  | CT_commit -> content.content.content.content
+  | _ -> failwith "extract_commit: not a commit"
+
+val test_commit_protection: {|crypto_bytes bytes|} -> message_protection_test -> ML bool
+let test_commit_protection #cb t =
+  let encryption_secret = hex_string_to_bytes t.encryption_secret in
+  let sender_data_secret = hex_string_to_bytes t.sender_data_secret in
+  let commit = hex_string_to_bytes t.commit in
+  let commit_pub = extract_public_message t.commit_pub in
+  let commit_priv = extract_private_message t.commit_priv in
+
+  let the_commit_pub = extract_commit (message_plaintext_to_message commit_pub) in
+  let the_commit_priv = extract_commit (extract_result (message_ciphertext_to_message 1 encryption_secret sender_data_secret commit_priv)) in
+
+  let the_commit_pub_ok = check_equal "commit_pub" (bytes_to_hex_string) (commit) ((ps_prefix_to_ps_whole ps_commit_nt).serialize the_commit_pub) in
+  let the_commit_priv_ok = check_equal "commit_priv" (bytes_to_hex_string) (commit) ((ps_prefix_to_ps_whole ps_commit_nt).serialize the_commit_priv) in
+
+  the_commit_pub_ok && the_commit_priv_ok
+
+val extract_application: {|bytes_like bytes|} -> authenticated_content_nt bytes -> ML bytes
+let extract_application #bl content =
+  match content.content.content.content_type with
+  | CT_application -> content.content.content.content
+  | _ -> failwith "extract_application: not a application"
+
+val test_application_protection: {|crypto_bytes bytes|} -> message_protection_test -> ML bool
+let test_application_protection #cb t =
+  let encryption_secret = hex_string_to_bytes t.encryption_secret in
+  let sender_data_secret = hex_string_to_bytes t.sender_data_secret in
+  let application = hex_string_to_bytes t.application in
+  let application_priv = extract_private_message t.application_priv in
+
+  let the_application_priv = extract_application (extract_result (message_ciphertext_to_message 1 encryption_secret sender_data_secret application_priv)) in
+
+  let the_application_priv_ok = check_equal "application_priv" (bytes_to_hex_string) (application) the_application_priv in
+
+  the_application_priv_ok
+
+val test_message_protection_one: message_protection_test -> ML bool
+let test_message_protection_one t =
+  match uint16_to_ciphersuite t.cipher_suite with
+  | ProtocolError s -> begin
+    IO.print_string ("Skipping one test because of missing ciphersuite: '" ^ s ^ "'\n");
+    true
+  end
+  | InternalError s -> begin
+    IO.print_string ("Internal error! '" ^ s ^ "'\n");
+    false
+  end
+  | Success cs -> begin
+    match cs with
+    | AC_mls_128_dhkemx25519_aes128gcm_sha256_ed25519
+    | AC_mls_128_dhkemp256_aes128gcm_sha256_p256 -> (
+      IO.print_string "(message protection: skipping one message protection test because AES-GCM is unavailable)\n";
+      true
+    )
+    | _ -> (
+      let cb = mk_concrete_crypto_bytes cs in
+      let proposal_ok = test_proposal_protection t in
+      let commit_ok = test_commit_protection t in
+      let application_ok = test_application_protection t in
+      proposal_ok && commit_ok && application_ok
+    )
+  end
+
+val test_message_protection: list message_protection_test -> ML bool
+let test_message_protection =
+  test_list "Message Protection" test_message_protection_one
